BitVec simplification

Auto/Embedding/LamBitVec.lean
@@ -4,13 +4,20 @@ import Std.Data.Fin.Lemmas
 
 namespace Auto.Embedding.Lam
 
-section BVTheorems
+namespace BitVec
 
   open Std.BitVec
   
   theorem ofNat_add (n a b : Nat) : (a + b)#n = a#n + b#n := by
     apply congrArg (f:=Std.BitVec.ofFin); apply Fin.eq_of_val_eq
     dsimp [Fin.ofNat']; rw [Nat.add_mod]; rfl
+  
+  theorem ofNat_toNat_lengthEq (bv : Std.BitVec n) : bv.toNat#n = bv := by
+    cases bv; case ofFin fin =>
+      cases fin; case mk val isLt =>
+        dsimp [Std.BitVec.toNat, Std.BitVec.ofNat]
+        apply congrArg; apply Fin.eq_of_val_eq
+        dsimp [Fin.ofNat']; rw [Nat.mod_eq_of_lt isLt]
   
   theorem ofNat_mod_pow2 (n a : Nat) : (a % (2 ^ n))#n = a#n := by
     apply congrArg (f:=Std.BitVec.ofFin); apply Fin.eq_of_val_eq
@@ -20,11 +27,17 @@ section BVTheorems
     apply congrArg (f:=Std.BitVec.ofFin); apply Fin.eq_of_val_eq
     dsimp [Fin.ofNat']; rw [Nat.mul_mod]; rfl
 
-end BVTheorems
+end BitVec
 
 theorem LamEquiv.bvofNat :
   LamEquiv lval lctx (.base (.bv n)) (.mkBvofNat n (.mkNatVal i)) (.base (.bvVal' n i)) :=
   ⟨.mkBvofNat (.ofBase (.ofNatVal' i)), .ofBase (.ofBvVal' n i), fun _ => rfl⟩
+
+theorem LamEquiv.bvofNat_bvtoNat_lengthEq
+  (wft : LamWF lval.toLamTyVal ⟨lctx, t, .base (.bv n)⟩) :
+  LamEquiv lval lctx (.base (.bv n)) (.mkBvofNat n (.mkBvUOp n (.bvtoNat n) t)) t :=
+  ⟨.mkBvofNat (.mkBvUOp (.ofBvtoNat n) wft), wft, fun lctxTerm => by
+    apply GLift.down.inj; apply BitVec.ofNat_toNat_lengthEq⟩
 
 theorem LamEquiv.bvofNat_nadd
   (wfa : LamWF lval.toLamTyVal ⟨lctx, a, .base .nat⟩)
@@ -34,6 +47,216 @@ theorem LamEquiv.bvofNat_nadd
     (.mkBvBinOp n (.bvadd n) (.mkBvofNat n a) (.mkBvofNat n b)) :=
   ⟨.mkBvofNat (.mkNatBinOp .ofNadd wfa wfb),
    .mkBvBinOp (.ofBvadd _) (.mkBvofNat wfa) (.mkBvofNat wfb), fun lctxTerm => by
-      apply GLift.down.inj; apply ofNat_add⟩
+      apply GLift.down.inj; apply BitVec.ofNat_add⟩
+
+theorem LamEquiv.bvofNat_nmul
+  (wfa : LamWF lval.toLamTyVal ⟨lctx, a, .base .nat⟩)
+  (wfb : LamWF lval.toLamTyVal ⟨lctx, b, .base .nat⟩) :
+  LamEquiv lval lctx (.base (.bv n))
+    (.mkBvofNat n (.mkNatBinOp .nmul a b))
+    (.mkBvBinOp n (.bvmul n) (.mkBvofNat n a) (.mkBvofNat n b)) :=
+  ⟨.mkBvofNat (.mkNatBinOp .ofNmul wfa wfb),
+   .mkBvBinOp (.ofBvmul _) (.mkBvofNat wfa) (.mkBvofNat wfb), fun lctxTerm => by
+      apply GLift.down.inj; apply BitVec.ofNat_mul⟩
+
+inductive BVCastType where
+  | ofNat : Nat → BVCastType
+  | ofInt : Nat → BVCastType
+  | none
+
+def LamTerm.applyBVCast (ct : BVCastType) (t : LamTerm) : LamTerm :=
+  match ct with
+  | .ofNat n => mkBvofNat n t
+  | .ofInt n => mkBvofInt n t
+  | .none    => t
+
+def LamTerm.pushBVCast (ct : BVCastType) (t : LamTerm) : LamTerm :=
+  match ct with
+  | .ofNat n =>
+    match t with
+    | .base (.ncst (.natVal i)) => .base (.bvcst (.bvVal n i))
+    | .app _ (.app _ (.base (.ncst .nadd)) lhs) rhs =>
+      mkBvBinOp n (.bvadd n) (pushBVCast (.ofNat n) lhs) (pushBVCast (.ofNat n) rhs)
+    | .app _ (.app _ (.base (.ncst .nmul)) lhs) rhs =>
+      mkBvBinOp n (.bvmul n) (pushBVCast (.ofNat n) lhs) (pushBVCast (.ofNat n) rhs)
+    | _ => mkBvofNat n t
+  -- Not implemented
+  | .ofInt n => mkBvofInt n t
+  | .none =>
+    match t with
+    | .lam s body => .lam s (pushBVCast .none body)
+    | .app _ (.base (.bvcst (.bvofNat n))) t' => pushBVCast (.ofNat n) t'
+    | .app _ (.base (.bvcst (.bvofInt n))) t' => pushBVCast (.ofInt n) t'
+    | .app s fn arg => .app s (pushBVCast .none fn) (pushBVCast .none arg)
+    | _ => t
+
+theorem LamTerm.maxEVarSucc_pushBVCast : maxEVarSucc (pushBVCast ct t) = maxEVarSucc t := by
+  generalize tl' : t.size = l; have tl : t.size ≤ l := by cases tl'; exact .refl
+  clear tl'
+  induction l generalizing t ct <;>
+    try apply False.elim (LamTerm.size_ne_zero (Nat.le_zero.mp tl))
+  case succ l IH =>
+    cases t <;> try (cases ct <;> rfl)
+    case base b =>
+      cases b <;> try (cases ct <;> rfl)
+      case ncst nc =>
+        cases nc <;> cases ct <;> rfl
+    case lam s body =>
+      cases ct <;> try apply Nat.max_zero_left
+      case none =>
+        dsimp [pushBVCast, maxEVarSucc]; apply IH
+        apply Nat.le_of_succ_le_succ tl
+    case app s fn arg =>
+      cases ct
+      case ofNat m =>
+        cases fn <;> try apply Nat.max_zero_left
+        case app s fn arg₁ =>
+          cases fn <;> try apply Nat.max_zero_left
+          case base b =>
+            cases b <;> try apply Nat.max_zero_left
+            case ncst nc =>
+              cases nc <;> (try apply Nat.max_zero_left) <;> (
+                dsimp [pushBVCast, maxEVarSucc]
+                rw [IH (t:=arg₁) (Nat.le_of_succ_le_succ (Nat.le_trans (Nat.le_trans
+                  LamTerm.size_app_gt_size_arg LamTerm.size_app_ge_size_fn) tl))]
+                rw [IH (t:=arg) (Nat.le_of_succ_le_succ (Nat.le_trans
+                  LamTerm.size_app_gt_size_arg tl))])              
+      case ofInt m => apply Nat.max_zero_left
+      case none =>
+        cases fn <;> try (
+          dsimp [maxEVarSucc, pushBVCast]; rw [IH (t:=arg) (Nat.le_of_succ_le_succ (
+            Nat.le_trans LamTerm.size_app_gt_size_arg tl))])
+        case base b =>
+          cases b <;> try (
+            dsimp [maxEVarSucc, pushBVCast]; rw [IH (t:=arg) (Nat.le_of_succ_le_succ (
+              Nat.le_trans LamTerm.size_app_gt_size_arg tl))])
+          case bvcst bvc =>
+            cases bvc <;> dsimp [maxEVarSucc, pushBVCast] <;> rw [IH (t:=arg) (Nat.le_of_succ_le_succ (
+                Nat.le_trans LamTerm.size_app_gt_size_arg tl))]
+            case bvofNat => rw [Nat.max, Nat.max_zero_left]
+            case bvofInt => rw [Nat.max, Nat.max_zero_left]
+        case lam s body =>
+          rw [IH (t:=body)]; apply Nat.le_of_succ_le_succ (Nat.le_trans _ tl)
+          apply LamTerm.size_app_ge_size_fn (fn:=.lam s body)
+        case app s fn arg =>
+          rw [IH (t:=.app s fn arg)]; rfl
+          apply Nat.le_of_succ_le_succ (Nat.le_trans _ tl)
+          apply LamTerm.size_app_gt_size_fn (fn:=.app s fn arg)
+
+theorem LamTerm.evarEquiv_pushBVCast : evarEquiv (fun t => pushBVCast ct t) := by
+  intro t t' heq; cases heq; apply maxEVarSucc_pushBVCast
+
+theorem LamEquiv.pushBVCast
+  (wft : LamWF lval.toLamTyVal ⟨lctx, LamTerm.applyBVCast ct t, s⟩) :
+  LamEquiv lval lctx s (t.applyBVCast ct) (t.pushBVCast ct) := by
+  generalize tl' : t.size = l; have tl : t.size ≤ l := by cases tl'; exact .refl
+  clear tl'
+  induction l generalizing t s ct lctx <;>
+    try apply False.elim (LamTerm.size_ne_zero (Nat.le_zero.mp tl))
+  case succ l IH =>
+    cases t
+    case atom n =>
+      cases ct <;> dsimp [LamTerm.pushBVCast] <;> apply LamEquiv.refl wft
+    case etom n =>
+      cases ct <;> dsimp [LamTerm.pushBVCast] <;> apply LamEquiv.refl wft
+    case base b =>
+      cases ct <;> try (dsimp [LamTerm.pushBVCast]; apply LamEquiv.refl wft)
+      case ofNat m =>
+        cases b <;> try (dsimp [LamTerm.pushBVCast]; apply LamEquiv.refl wft)
+        case ncst nc =>
+          cases nc <;> dsimp [LamTerm.pushBVCast, LamTerm.applyBVCast] <;> try apply LamEquiv.refl wft
+          cases wft.getFn.getBase.getBvcst; apply LamEquiv.bvofNat
+    case bvar n =>
+      cases ct <;> dsimp [LamTerm.pushBVCast] <;> apply LamEquiv.refl wft
+    case lam s' body =>
+      cases ct <;> try (dsimp [LamTerm.pushBVCast]; apply LamEquiv.refl wft)
+      case none =>
+        dsimp [LamTerm.pushBVCast, LamTerm.applyBVCast]
+        cases wft
+        case ofLam s'' wfBody =>
+          apply LamEquiv.ofLam; apply IH (ct:=.none) (t:=body) wfBody
+          apply Nat.le_of_succ_le_succ tl
+    case app s' fn arg =>
+      cases ct
+      case ofNat m =>
+        cases fn <;> try (dsimp [LamTerm.pushBVCast]; apply LamEquiv.refl wft)
+        case app s'' fn arg₁ =>
+          cases fn <;> try (dsimp [LamTerm.pushBVCast]; apply LamEquiv.refl wft)
+          case base b =>
+            cases b <;> try (dsimp [LamTerm.pushBVCast]; apply LamEquiv.refl wft)
+            case ncst nc =>
+              cases nc <;> dsimp [LamTerm.pushBVCast] <;> try apply LamEquiv.refl wft
+              case nadd =>
+                cases wft.getFn.getBase.getBvcst
+                have wfnadd := wft.getArg
+                cases wfnadd.getFn.getFn.getBase.getNcst
+                have wfl := wfnadd.getFn.getArg; have wfr := wfnadd.getArg
+                dsimp [LamTerm.applyBVCast]
+                apply LamEquiv.trans (LamEquiv.bvofNat_nadd wfl wfr)
+                apply LamEquiv.congr (LamEquiv.congrArg (.ofBase (.ofBvadd' _)) ?eql) ?eqr
+                case eql =>
+                  apply IH (ct:=.ofNat m) (t:=arg₁) (.mkBvofNat wfl)
+                  apply Nat.le_of_succ_le_succ (Nat.le_trans (Nat.le_trans
+                    LamTerm.size_app_gt_size_arg LamTerm.size_app_ge_size_fn) tl)
+                case eqr =>
+                  apply IH (ct:=.ofNat m) (t:=arg) (.mkBvofNat wfr)
+                  apply Nat.le_of_succ_le_succ (Nat.le_trans LamTerm.size_app_gt_size_arg tl)
+              case nmul =>
+                cases wft.getFn.getBase.getBvcst
+                have wfnadd := wft.getArg
+                cases wfnadd.getFn.getFn.getBase.getNcst
+                have wfl := wfnadd.getFn.getArg; have wfr := wfnadd.getArg
+                dsimp [LamTerm.applyBVCast]
+                apply LamEquiv.trans (LamEquiv.bvofNat_nmul wfl wfr)
+                apply LamEquiv.congr (LamEquiv.congrArg (.ofBase (.ofBvmul' _)) ?eql) ?eqr
+                case eql =>
+                  apply IH (ct:=.ofNat m) (t:=arg₁) (.mkBvofNat wfl)
+                  apply Nat.le_of_succ_le_succ (Nat.le_trans (Nat.le_trans
+                    LamTerm.size_app_gt_size_arg LamTerm.size_app_ge_size_fn) tl)
+                case eqr =>
+                  apply IH (ct:=.ofNat m) (t:=arg) (.mkBvofNat wfr)
+                  apply Nat.le_of_succ_le_succ (Nat.le_trans LamTerm.size_app_gt_size_arg tl)
+      case ofInt m => dsimp [LamTerm.pushBVCast]; apply LamEquiv.refl wft
+      case none =>
+        cases fn <;> try (
+          dsimp [LamTerm.pushBVCast]; apply LamEquiv.congrArg wft.getFn
+          apply IH (ct:=.none) wft.getArg; apply Nat.le_of_succ_le_succ (Nat.le_trans
+            LamTerm.size_app_gt_size_arg tl))
+        case base b =>
+          cases b <;> try (
+            apply LamEquiv.congrArg wft.getFn (IH (ct:=.none) wft.getArg _)
+            apply Nat.le_of_succ_le_succ (Nat.le_trans LamTerm.size_app_gt_size_arg tl))
+          case bvcst bvc =>
+            cases bvc <;> try (
+              apply LamEquiv.congrArg wft.getFn (IH (ct:=.none) wft.getArg _)
+              apply Nat.le_of_succ_le_succ (Nat.le_trans LamTerm.size_app_gt_size_arg tl))
+            case bvofNat m =>
+              cases wft.getFn.getBase.getBvcst
+              apply IH (ct:=.ofNat m) (t:=arg) wft
+              apply Nat.le_of_succ_le_succ (Nat.le_trans LamTerm.size_app_gt_size_arg tl)
+            case bvofInt m =>
+              cases wft.getFn.getBase.getBvcst
+              apply IH (ct:=.ofInt m) (t:=arg) wft
+              apply Nat.le_of_succ_le_succ (Nat.le_trans LamTerm.size_app_gt_size_arg tl)
+        case lam s' body =>
+          dsimp [LamTerm.applyBVCast]; apply LamEquiv.congr
+          case eFn =>
+            apply IH (ct:=.none) (t:=.lam s' body) wft.getFn
+            apply Nat.le_of_succ_le_succ (Nat.le_trans LamTerm.size_app_gt_size_fn tl)
+          case eArg =>
+            apply IH (ct:=.none) (t:=arg) wft.getArg
+            apply Nat.le_of_succ_le_succ (Nat.le_trans LamTerm.size_app_gt_size_arg tl)
+        case app s'' fn arg₁ =>
+          dsimp [LamTerm.applyBVCast]; apply LamEquiv.congr
+          case eFn =>
+            apply IH (ct:=.none) (t:=.app s'' fn arg₁) wft.getFn
+            apply Nat.le_of_succ_le_succ (Nat.le_trans LamTerm.size_app_gt_size_fn tl)
+          case eArg =>
+            apply IH (ct:=.none) (t:=arg) wft.getArg
+            apply Nat.le_of_succ_le_succ (Nat.le_trans LamTerm.size_app_gt_size_arg tl)
+
+theorem LamGenConv.pushBVCast : LamGenConv lval (fun t => LamTerm.pushBVCast .none t) := by
+  intros t₁ t₂ heq lctx rty wf; cases heq
+  apply LamEquiv.pushBVCast (ct:=.none) wf
 
 end Auto.Embedding.Lam
